monadproofs/proofs/demoprf.v
@@ -79,6 +79,7 @@ Section with_Sigma.
   Qed.
 
 
+  (* TODO: add lambdap and lambdStructObjOwnership arguments *)
   Definition ThreadR (lamStructName: core.name) (P Q : mpred) : Rep. Proof using. Admitted.
   
   Definition ThreadConstructor (lamStructName: core.name) (this:ptr): WpSpec mpredI val val :=
@@ -94,6 +95,10 @@ Section with_Sigma.
     
     \post this |-> ThreadR lamStructName taskPre taskPost.
 
+  Definition ThreadDtor (lamStructName: core.name) (this:ptr): WpSpec mpredI val val :=
+    \pre{taskPre taskPost} this |-> ThreadR lamStructName taskPre taskPost
+    \post emp.
+  
   Definition fork_start (lamStructName: core.name) (this:ptr): WpSpec mpredI val val :=
     \prepost{P Q} this |-> ThreadR lamStructName P Q
     \pre P
@@ -106,13 +111,13 @@ Section with_Sigma.
   cpp.spec "parallel_gcd_lcm(const unsigned int&, const unsigned int&, unsigned int&, unsigned int&)" as pgl with
       (
         \arg{ap} "a" (Vref ap)
-        \prepost{(qa:Qp) (av:N)} ap |-> primR "int" qa av
+        \prepost{(qa:Qp) (av:N)} ap |-> primR "unsigned int" qa av
         \arg{bp} "b" (Vref bp)
-        \prepost{(qb:Qp) (bv:N)} bp |-> primR "int" qb bv
+        \prepost{(qb:Qp) (bv:N)} bp |-> primR "unsigned int" qb bv
         \arg{gp} "gcd_result" (Vref gp)
-        \pre{garbage1:N} gp |-> primR "int" 1 garbage1
+        \pre{garbage1:N} gp |-> primR "unsigned int" 1 garbage1
         \arg{lp} "lcm_result" (Vref lp)
-        \pre{garbage2:N} lp |-> primR "int" 1 garbage2
+        \pre{garbage2:N} lp |-> primR "unsigned int" 1 garbage2
         \post emp
       ).
 
@@ -124,12 +129,12 @@ Section with_Sigma.
 
   cpp.spec "gcd(const unsigned int&, const unsigned int&, unsigned int&)" as gcd2_spec with (
         \arg{ap} "a" (Vref ap)
-        \prepost{(qa:Qp) (av:N)} ap |-> primR "int" qa av
+        \prepost{(qa:Qp) (av:N)} ap |-> primR "unsigned int" qa av
         \arg{bp} "b" (Vref bp)
-        \prepost{(qb:Qp) (bv:N)} bp |-> primR "int" qb bv
+        \prepost{(qb:Qp) (bv:N)} bp |-> primR "unsigned int" qb bv
         \arg{gp} "gcd_result" (Vref gp)
-        \pre{garbage1:N} gp |-> primR "int" 1 garbage1
-        \post gp |-> primR "int" 1 (Z.gcd av bv)
+        \pre{garbage1:N} gp |-> primR "unsigned int" 1 garbage1
+        \post gp |-> primR "unsigned int" 1 (Z.gcd av bv)
       ).
 
   Definition thread_constructor (lamStructTyName: core.name) :=
@@ -143,33 +148,165 @@ Section with_Sigma.
     |}
     (ThreadConstructor lamStructTyName).
 
+  Definition thread_destructor (lamStructTyName: core.name) :=
+  specify
+    {|
+      info_name :=
+        Nscoped (Ninst "Thread" [Atype (Tnamed lamStructTyName)]) Ndtor;
+      info_type :=
+        tDtor (Ninst "Thread" [Atype (Tnamed lamStructTyName)])
+    |}
+    (ThreadDtor lamStructTyName).
+  
+  (*TODO: rename to just start? *)
+  Definition thread_fork_start (lamStructTyName: core.name) :=
+  specify
+    {|
+      info_name :=
+        Nscoped (Ninst "Thread" [Atype (Tnamed lamStructTyName)]) (Nfunction function_qualifiers.N "fork_start" []);
+      info_type :=
+        tMethod (Ninst "Thread" [Atype (Tnamed lamStructTyName)]) QM "void" []
+    |}
+    (fork_start lamStructTyName).
+
+  Definition thread_fork_join (lamStructTyName: core.name) :=
+  specify
+    {|
+      info_name :=
+        Nscoped (Ninst "Thread" [Atype (Tnamed lamStructTyName)]) (Nfunction function_qualifiers.N "join" []);
+      info_type :=
+        tMethod (Ninst "Thread" [Atype (Tnamed lamStructTyName)]) QM "void" []
+    |}
+    (join lamStructTyName).
+  
+  cpp.spec "Thread<parallel_gcd_lcm(const unsigned int&, const unsigned int&, unsigned int&, unsigned int&)::@0>::fork_start()"
+           as ff with (fork_start "parallel_gcd_lcm(const unsigned int&, const unsigned int&, unsigned int&, unsigned int&)::@0").
   Lemma par: denoteModule module |-- pgl.
   Proof using.
     verify_spec'.
     go.
   Abort.
+
+  Definition thread_class_specs lamStructName :=
+    thread_constructor lamStructName **
+    thread_fork_start lamStructName **
+    thread_fork_join lamStructName **
+    thread_destructor lamStructName.
    
   Existing Instance UNSAFE_read_prim_cancel.
+  #[global] Instance : forall ty P Q, Observe (reference_toR (Tnamed ty)) (ThreadR ty P Q).
+  Proof. Admitted.
 
-  Lemma par: denoteModule module ** (thread_constructor "parallel_gcd_lcm(const unsigned int&, const unsigned int&, unsigned int&, unsigned int&)::@0") ** gcd2_spec |-- pgl.
+  Lemma primr_split (p:ptr) ty (q:Qp) v :
+    p|-> primR ty (cQpc q) v -|- (p |-> primR ty (cQpc q/2) v) ** p |-> primR ty (cQpc q/2) v.
   Proof using.
+    unfold cQpc.
+    rewrite -> cfractional_split_half with (R := fun q => primR ty q v).
+    2:{ exact _. }
+    rewrite _at_sep.
+    f_equiv; f_equiv; f_equiv;
+    simpl;
+      rewrite cQp.scale_mut;
+      f_equiv;
+    destruct q; simpl in *;
+      solveQpeq;
+      solveQeq.
+  Qed.
+  #[global] Instance obss (pp:ptr) ty P Q: Observe (reference_to (Tnamed (Ninst "Thread" [Atype (Tnamed ty)])) pp) (pp |-> ThreadR ty P Q).
+  Proof. Admitted.
+  
+  Lemma par: denoteModule module ** (thread_class_specs "parallel_gcd_lcm(const unsigned int&, const unsigned int&, unsigned int&, unsigned int&)::@0") ** gcd2_spec |-- pgl.
+  Proof using.
+    unfold thread_class_specs.
     verify_spec'.
     slauto.
-    aggregateRepPieces a.
+    aggregateRepPieces gcdLambda_addr.
     go.
     
     fold cQpc.
-    (* TODO: pick a better name *)
-    iExists (gp |-> intR 1%Qp garbage1 ** ap |-> intR (qa/3) av ** bp |-> intR (qb/3) bv).
-    iExists (gp |-> intR 1%Qp (Z.gcd av bv) ** ap |-> intR (qa/3) av ** bp |-> intR (qb/3) bv).
+    (* TODO: pick a better name for gp. TODO. replace unintR with primR  *)
+    iExists (gp |-> uintR 1%Qp garbage1 ** ap |-> uintR (qa/2) av ** bp |-> uintR (qb/2) bv).
+    iExists (gp |-> uintR 1%Qp (Z.gcd av bv) ** ap |-> uintR (qa/2) av ** bp |-> uintR (qb/2) bv).
     go.
     iSplitL "".
     { verify_spec'.
       go.
     }
     iIntrosDestructs.
+    do 6 run1.
+  #[global] Instance : forall ty , LearnEq2 (ThreadR ty) := ltac:(solve_learnable).
+    step.
+    step.
+    step.
+    fold cQpc.
+    rewrite (primr_split ap).
+    rewrite (primr_split bp).
+    go.
+    Compute (Z.gcd 0 0).
+    Search 0%Z (Z.gcd _ _)%Z.
+    pose proof (Z.gcd_nonneg av bv).
+    pose proof (Z.gcd_eq_0 av bv).
+    assert (0< av \/ 0< bv)%N as Heq.
+    admit.
+    provePure.
+    destruct Heq; try lia.
+    go.
+    (* TODO: generalize *)
+  cpp.spec (Nscoped 
+              "parallel_gcd_lcm(const unsigned int&, const unsigned int&, unsigned int&, unsigned int&)::@0" Ndtor)  as lamdestr
+                                                                                                                          inline.
+  go.
+     (fun (this:ptr) => \pre ThreadR
+    go.
+    
+    lia.
+    go.
+    Search Z.gcd iff.
+    pose proof (Z.gcd_nonneg).
+    
+    step.
+    step.
+    step.
+    Qeq.
+    apply Qpeq; unfold toQ; unfold makeQp; simpl.
+    f_equiv.
+    Search Qp_to_Qc.
+   Search Qcanon.this.
+  repeat rewrite Qred_correct.
+
+    solveQpeq.
+    f_equiv.
+    rewrite Qred_correct.
+    go.
+    Set  Printing All.
+    go.
+    Search (/2)%Qp.
+    Search cQp.scale cQp.mut.
+    reflexivity.
+    go.
+    Search CFractional (1/2)%Qp.
+    Seach 
+  Search cQp.mut primR.
+    do 5  run1.
+    step.
+    step.
+    go.
+    reference_to "Thread<parallel_gcd_lcm(const unsigned int&, const unsigned int&, unsigned int&, unsigned int&)::@0>" t1_addr
+   reference_to "parallel_gcd_lcm(const unsigned int&, const unsigned int&, unsigned int&, unsigned int&)::@0" t1_addr                                                                                                                        
+    do 4 run1.
+    Set Nested Proofs Allowed.
+    go.
+    obs_elim
     slauto.
-    const.
+    run1.
+    run1.
+    run1.
+    run1.
+    
+    observe_elim_cancel
+    slauto.
+    go.
+    Search primR Learnable.
     go.
     slauto.
     go.
